* Chapter 1.2 Exercise Solutions

** Exercise 1
*** 1a

| P | Q | (¬P ∨ Q) |
|---+---+----------|
| F | F | T        |
| F | T | T        |
| T | F | F        |
| T | T | T        |

*** 1b

| S | G | (S ∨ G) ∧ (¬S ∨ ¬G) |
|---+---+---------------------|
| F | F | F                   |
| F | T | T                   |
| T | F | T                   |
| T | T | F                   |

** Exercise 2
*** 2a

| P | Q | ¬[P ∧ (Q ∨ ¬P)] |
|---+---+-----------------|
| F | F | T               |
| F | T | T               |
| T | F | T               |
| T | T | F               |

*** 2b

| P | Q | R | (P ∨ Q) ∧ (¬P ∨ R) |
|---+---+---+--------------------|
| F | F | F | F                  |
| F | F | T | F                  |
| F | T | F | T                  |
| F | T | T | T                  |
| T | F | F | F                  |
| T | F | T | T                  |
| T | T | F | F                  |
| T | T | T | T                  |

** Exercise 3
*** 3a

| P | Q | P + Q |
|---+---+-------|
| F | F | F     |
| F | T | T     |
| T | F | T     |
| T | T | F     |

*** 3b

| P | Q | (P ∨ Q) ∧ ¬(P ∧ Q) |
|---+---+--------------------|
| F | F | F                  |
| F | T | T                  |
| T | F | T                  |
| T | T | F                  |

** Exercise 4

¬(¬P ∧ ¬Q)

| P | Q | (P ∨ Q) | ¬(¬P ∧ ¬Q) |
|---+---+---------+------------|
| F | F | F       | F          |
| F | T | T       | T          |
| T | F | T       | T          |
| T | T | T       | T          |

** Exercise 5

*** 5a

| P | Q | P ↓ Q |
|---+---+-------|
| F | F | T     |
| F | T | F     |
| T | F | F     |
| T | T | F     |

*** 5b
¬P ∧ ¬Q

*** 5c
- ¬P is equivalent to P ↓ P
- P ∨ Q is equivalent to (P ↓ Q) ↓ (P ↓ Q)
- P ∧ Q is equivalent to (P ↓ P) ↓ (Q ↓ Q)

** Exercise 6

*** 6a

| P | Q | P \vert Q |
|---+---+-----------|
| F | F | T         |
| F | T | T         |
| T | F | T         |
| T | T | F         |

*** 6b

- ¬(P ∧ Q) is equivalent to P | Q

*** 6c

- ¬P is equivalent to P | P
- P ∨ Q is equivalent to (P | P) | (Q | Q)
- P ∧ Q is equivalent to (P | Q) | (P | Q)

** Exercise 7

Let P = Pete will win the math prize
    J = Jame will win the math prize
    C = Pete will win the chemistry prize

| P | J | C | ¬(P ∧ J) | (P ∨ C) | J | C |
|---+---+---+----------+---------+---+---|
| F | F | F | T        | F       | F | F |
| F | F | T | T        | T       | F | T |
| F | T | F | T        | F       | T | F |
| F | T | T | T        | T       | T | T |
| T | F | F | T        | T       | F | F |
| T | F | T | T        | T       | F | T |
| T | T | F | F        | T       | T | F |
| T | T | T | F        | T       | T | T |

C is true whenever all premises are true, therefore argument is valid.

Let B = Main course will be beef
    F = Main course will be fish
    P = Vegetable will be peas
    C = Vegetable will be corn

B ∨ F
P ∨ C
¬(F ∧ C)
--------
(B ∧ P)

| B | F | P | C | B ∨ F | P ∨ C | ¬(F ∧ C) | B ∧ P |    |
|---+---+---+---+-------+-------+----------+-------+----|
| F | F | F | F | F     | F     | T   F    | F     |    |
| F | F | F | T | F     | T     | T   F    | F     |    |
| F | F | T | F | F     | T     | T   F    | F     |    |
| F | F | T | T | F     | T     | T   F    | F     |    |
| F | T | F | F | T     | F     | T   F    | F     |    |
| F | T | F | T | T     | T     | F   T    | F     |    |
| F | T | T | F | T     | T     | T   F    | F     | :( |
| F | T | T | T | T     | T     | F   T    | F     |    |
| T | F | F | F | T     | F     | T   F    | F     |    |
| T | F | F | T | T     | T     | T   F    | F     | :( |
| T | F | T | F | T     | T     | T   F    | T     | :) |
| T | F | T | T | T     | T     | T   F    | T     | :) |
| T | T | F | F | T     | F     | T   F    | F     |    |
| T | T | F | T | T     | T     | F   T    | F     |    |
| T | T | T | F | T     | T     | T   F    | T     | :) |
| T | T | T | T | T     | T     | F   T    | T     |    |

There exists cases where all premises are true but conclusion is false therefore this is an invalid argument.

Let J = John is telling the truth
    B = Bill is telling the truth
    S = Sam is telling the truth

| J | B | S | J ∨ B | (¬S ∨ ¬B) | (J ∨ ¬S) |    |
|---+---+---+-------+-----------+----------+----|
| F | F | F | F     | T         | T        |    |
| F | F | T | F     | T         | F        |    |
| F | T | F | T     | T         | T        | :) |
| F | T | T | T     | F         | F        |    |
| T | F | F | T     | T         | T        |    |
| T | F | T | T     | T         | T        | :) |
| T | T | F | T     | T         | T        | :) |
| T | T | T | T     | F         | T        |    |

Conclusion is true when premises are true, therefore valid argument.

Let S = Sales go up
    X = Expenses go up
    B = Boss will be happy


| S | X | B | (S ∧ B) ∨ (X ∧ ¬B) | S \vert X |
|---+---+---+--------------------+-----------|
| F | F | F | F                  | T         |
| F | F | T | F                  | T         |
| F | T | F | T                  | F         |
| F | T | T | F                  | F         |
| T | F | F | F                  | F         |
| T | F | T | T                  | F         |
| T | T | F | T                  | F         |
| T | T | T | T                  | F         |

Argument is invalid because conclusion isn't always true when premise is true.

** Exercise 8

| P | Q | (P ∧ Q) ∨ (¬P ∧ ¬Q) | ¬P ∨ Q | (P ∨ ¬Q) ∧ (Q ∨ ¬P) | ¬(P ∨ Q) | (Q ∧ P) ∨ ¬P |
|---+---+---------------------+--------+---------------------+----------+--------------|
| F | F | T                   | T      | T                   | T        | T            |
| F | T | F                   | T      | F                   | F        | T            |
| T | F | F                   | F      | F                   | F        | F            |
| T | T | T                   | T      | T                   | F        | T            |

(Q ∧ P) ∨ ¬P and
(P ∨ ¬Q) ∧ (Q ∨ ¬P) are equivalent.

¬P ∨ Q and
(Q ∧ P) ∨ ¬P are equivalent.

** Exercise 9

a) Neither.
b) Contradiction.
c) Tautology.
d) Tautology.

** Exercise 10

*** 10a
DeMorgan's second law is ¬(P ∨ Q) is equivalent to ¬P ∧ ¬Q.

| P | Q | ¬(P ∨ Q) | ¬P ∧ ¬Q |
|---+---+----------+---------|
| F | F | T        | T       |
| F | T | F        | F       |
| T | F | F        | F       |
| T | T | F        | F       |

*** 10b
The distributive laws are:
- P ∧ (Q ∨ R) is equivalent to (P ∧ Q) ∨ (P ∧ R)

| P | Q | R | P ∧ (Q ∨ R) | (P ∧ Q) ∨ (P ∧ R) |
|---+---+---+-------------+-------------------|
| F | F | F | F           | F                 |
| F | F | T | F           | F                 |
| F | T | F | F           | F                 |
| F | T | T | F           | F                 |
| T | F | F | F           | F                 |
| T | F | T | T           | T                 |
| T | T | F | T           | T                 |
| T | T | T | T           | T                 |

- P ∨ (Q ∧ R) is equivalent to (P ∨ Q) ∧ (P ∨ R)

| P | Q | R | P ∨ (Q ∧ R) | (P ∨ Q) ∧ (P ∨ R) |
|---+---+---+-------------+-------------------|
| F | F | F | F           | F                 |
| F | F | T | F           | F                 |
| F | T | F | F           | F                 |
| F | T | T | T           | T                 |
| T | F | F | T           | T                 |
| T | F | T | T           | T                 |
| T | T | F | T           | T                 |
| T | T | T | T           | T                 |

** Exercise 11

*** 11 a
¬(¬P ∧ ¬Q)
¬¬P ∨ ¬¬Q  (DeMorgan's law)
P ∨ Q      (double negation law)
P ∨ Q

*** 11 b
(P ∧ Q) ∨ (P ∧ ¬Q)
P ∧ (Q ∨ ¬Q)  (DeMorgan's law - in reverse)
P             (tautology law)

*** 11 c
¬(P ∧ ¬Q) ∨ (¬P ∧ Q)
¬P ∨ ¬¬ Q ∨ (¬P ∧ Q)  (DeMorgan's law)
¬P ∨ Q ∨ (¬P ∧ Q)     (double negation law)
¬P ∨ (Q ∨ (Q ∧ ¬P))   (associativity law & rearrange)
¬P ∨ Q                (absorption law)

** Exercise 12

*** 12 a
¬(¬P ∨ Q) ∨ (P ∧ ¬R)
(¬¬P ∧ ¬Q) ∨ (P ∧ ¬R)  (DeMorgan's law)
(P ∧ ¬Q) ∨ (P ∧ ¬R)    (double negation law)
P ∧ (¬Q ∨ ¬R)          (distributive law)

*** 12 b
¬(¬P ∧ Q) ∨ (P ∧ ¬R)
(¬¬P ∨ Q) ∨ (P ∧ ¬R)  (DeMorgan's law)
(P ∨ Q) ∨ (P ∧ ¬R)    (double negation law)
Q ∨ (P ∨ (P ∧ ¬R))    (associativity law & rearrange)
Q ∨ P                 (absorption law)

*** 12 c
(P ∧ R) ∨ [¬R ∧ (P ∨ Q)]
(P ∧ R) ∨ [(¬R ∧ P) ∨ (¬R ∧ Q)]  (distributive law)
((P ∧ R) ∨ (P ∧ ¬R)) ∨ (¬R ∧ Q)  (associativity law & rearrange)
(P ∧ (R ∨ ¬R)) ∨ (¬R ∧ Q)        (distributive law)
P ∨ (¬R ∧ Q)                     (tautology law)

** Exercise 13

According to the double negation law, we know that:
  ¬¬(P ∧ Q) is equivalent to (P ∧ Q)
According to DeMorgan's first law, we can simplify this to:
  ¬(¬P ∨ ¬Q) is equivalent to (P ∧ Q)
We can use the double negation law again: 
  ¬(¬P ∨ ¬Q) is equivalent to (¬¬P ∧ ¬¬Q)
And if we perform the following substitution:
  Let R = ¬P
      S = ¬Q
We get:
  ¬(R ∨ S) is equivalent to (¬R ∧ ¬S)

Which is DeMorgan's second law.

** Exercise 14

[P ∧ (Q ∧ R)] ∧ S
[(P ∧ Q) ∧ R] ∧ S  (associativity law)
(P ∧ Q) ∧ (R ∧ S)  (associativity law)

** Exercise 15
There will be 2^n lines.

** Exercise 16
P ∨ ¬Q

** Exercise 17
(P ∨ Q) ∧ ¬(P ∧ Q)

** Exercise 18
If the conclusion of an argument is a tautology, then you can say that the
argument is valid, because the conclusion will always be true whenever the
premises are true.

If the conclusion of an argument is a contradiction, then you can say that the
argument is invalid, as the conclusion will always be false whenever the
premises are true.

If one of the premises of an argument is a contradiction or tautology, you
cannot say anything about the validity of the argument (either valid or
invalid).
