* Chapter 1.5 Exercise Solutions

** Exercise 1
** Exercise 2
** Exercise 3
** Exercise 4
*** 4a

Let S = "Sales will go up"
    X = "Expenses will go up"
    B = "Boss will be happy"

S ∨ X
S → B
X → ¬B
------
¬(S ∧ X)

| S | X | B | ¬B | S ∨ X | S → B | X → ¬B | ¬(S ∧ X) | Valid |
|---+---+---+----+-------+-------+--------+----------+-------|
| F | F | F | T  | F     | T     | T      | T        |       |
| F | F | T | F  | F     | T     | T      | T        |       |
| F | T | F | T  | T     | T     | T      | T        | y     |
| F | T | T | F  | T     | T     | F      | T        |       |
| T | F | F | T  | T     | F     | T      | T        |       |
| T | F | T | F  | T     | T     | T      | T        | y     |
| T | T | F | T  | T     | F     | T      | F        |       |
| T | T | T | F  | T     | T     | F      | F        |       |

Conclusion is true whenever all premises are true, therefore argument is valid.

*** 4b

Let T = "Tax rate will go up"
    U = "Unemployment rate will go up"
    R = "There will be a recession"
    G = "GNP goes up"

T ∧ U → R
G → ¬R
G ∧ T
----------
¬U

| T | U | R | G | T ∧ U | (T ∧ U) → R | G → ¬R | G ∧ T | ¬U | Valid |
|---+---+---+---+-------+-------------+--------+-------+----+-------|
| F | F | F | F | F     | T           | T      | F     | T  |       |
| F | F | F | T | F     | T           | T      | F     | T  |       |
| F | F | T | F | F     | T           | T      | F     | T  |       |
| F | F | T | T | F     | T           | F      | F     | T  |       |
| F | T | F | F | F     | T           | T      | F     | F  |       |
| F | T | F | T | F     | T           | T      | F     | F  |       |
| F | T | T | F | F     | T           | T      | F     | F  |       |
| F | T | T | T | F     | T           | F      | F     | F  |       |
| T | F | F | F | F     | T           | T      | F     | T  |       |
| T | F | F | T | F     | T           | T      | T     | T  | y     |
| T | F | T | F | F     | T           | T      | F     | T  |       |
| T | F | T | T | F     | T           | F      | T     | T  |       |
| T | T | F | F | T     | F           | T      | F     | F  |       |
| T | T | F | T | T     | F           | T      | T     | F  |       |
| T | T | T | F | T     | T           | T      | F     | F  |       |
| T | T | T | T | T     | T           | F      | T     | F  |       |

Conclusion is true whenever all premises are true, therefore argument is valid.

*** 4c

Let W = "The warning light will come on"
    P = "The pressure is too high"
    R = "Relief valve is clogged"
    
W <-> (P ∧ R)
¬R
-------------
W <-> P

| W | P | R | P ∧ R | W <-> (P ∧ R) | ¬R | W <-> P | Valid |
|---+---+---+-------+---------------+----+---------+-------|
| F | F | F | F     | T             | T  | T       | y     |
| F | F | T | F     | T             | F  | T       |       |
| F | T | F | F     | T             | T  | F       | n     |
| F | T | T | T     | F             | F  | F       |       |
| T | F | F | F     | F             | T  | F       |       |
| T | F | T | F     | F             | F  | F       |       |
| T | T | F | F     | F             | T  | T       |       |
| T | T | T | T     | T             | F  | T       |       |

Conclusion is not true whenever all premises are true, therefore argument is not valid.

** Exercise 5
*** 5a
Goal: (P ∧ Q) ∨ (¬P ∧ ¬Q)

| Step                                                          | Law used          |
|---------------------------------------------------------------+-------------------|
| P <-> Q                                                       |                   |
| (P -> Q) ∧ (Q -> P)                                           | definition of <-> |
| (¬P ∨ Q) ∧ (¬Q ∨ P)                                           | conditional law   |
| ((¬P ∨ Q) ∧ (¬Q ∨ P)) ∧ (P ∨ ¬P)                              | tautology law     |
| ((¬P ∨ Q) ∧ (P ∨ ¬P)) ∧ (¬Q ∨ P)                              | commutative law   |
| ((¬P ∨ Q) ∧ (¬P ∨ P)) ∧ (¬Q ∨ P)                              | commutative law   |
| (¬P ∨ (Q ∧ P)) ∧ (¬Q ∨ P)                                     | distributive law  |
| (¬P ∧ (¬Q ∨ P)) ∨ ((Q ∧ P) ∧ (¬Q ∨ P))                        | distributive law  |
| ((¬P ∧ ¬Q) ∨ (¬P ∧ P)) ∨ ((Q ∧ P) ∧ (¬Q ∨ P))                 | distributive law  |
| (¬P ∧ ¬Q) ∨ ((Q ∧ P) ∧ (¬Q ∨ P))                              | contradiction law |
| [(¬P ∧ ¬Q) ∨ (Q ∧ P)] ∧ [(¬P ∧ ¬Q) ∨ (¬Q ∨ P)]                | distributive law  |
| [(¬P ∧ ¬Q) ∨ (Q ∧ P)] ∧ [ (¬P ∨ (¬Q ∨ P)) ∧ (¬Q ∨ (¬Q ∨ P)) ] | distributive law  |
| [(¬P ∧ ¬Q) ∨ (Q ∧ P)] ∧ [ (¬P ∨ (P ∨ ¬Q)) ∧ (¬Q ∨ (¬Q ∨ P)) ] | commutative law   |
| [(¬P ∧ ¬Q) ∨ (Q ∧ P)] ∧ [ ((¬P ∨ P) ∨ ¬Q) ∧ ((¬Q ∨ ¬Q) ∨ P) ] | associativity law |
| [(¬P ∧ ¬Q) ∨ (Q ∧ P)] ∧ [ (((¬Q ∨ ¬Q) ∨ P) ]                  | tautology law     |
| (¬P ∧ ¬Q) ∨ (Q ∧ P)                                           | tautology law     |
| (P ∧ Q) ∨ (¬P ∧ ¬Q)                                           | commutative law   |

Therefore P <-> Q is equivalent to (P ∧ Q) ∨ (¬P ∧ ¬Q).

*** 5b
Goal: P → (Q ∨ R)

| Step                | Law used                         |
|---------------------+----------------------------------|
| (P → Q) ∨ (P → R)   |                                  |
| (¬P ∨ Q) ∨ (¬P ∨ R) | conditional law                  |
| (¬P ∨ ¬P) ∨ (Q ∨ R) | associative and commutative laws |
| ¬P ∨ (Q ∨ R)        | idempotent law                   |
| P → (Q ∨ R)         | conditional law                  |

Therefore (P → Q) ∨ (P → R) is equivalent to P → (Q ∨ R).

** Exercise 6

*** 6a

Goal: (P ∨ Q) → R

| Step                             | Law used         |
|----------------------------------+------------------|
| (P → R) ∧ (Q → R)                |                  |
| (¬P ∨ R) ∧ (¬Q ∨ R)              | conditional law  |
| [(¬P ∨ R) ∧ ¬Q] ∨ [(¬P ∨ R) ∧ R] | distributive law |
| [(¬P ∨ R) ∧ ¬Q] ∨ R              | absorption law   |
| [(¬P ∧ ¬Q) ∨ (R ∧ ¬Q)] ∨ R       | distributive law |
| (¬P ∧ ¬Q) ∨ [(R ∧ ¬Q) ∨ R]       | associative law  |
| (¬P ∧ ¬Q) ∨ R                    | absorption law   |
| ¬(P ∨ Q) ∨ R                     | DeMorgan's law   |
| (P ∨ Q) → R                      | conditional law  |

Therefore (P → R) ∧ (Q → R) is equivalent to (P ∨ Q) → R.

*** 6b

Know that (P → R) ∧ (Q → R) is equivalent to (P ∨ Q) → R.

So formulate that (P -> R) ∨ (Q -> R) is equivalent to (P ∧ Q) → R.

Goal: (P ∧ Q) → R

| Step                | Law used        |
|---------------------+-----------------|
| (P → R) ∨ (Q → R)   |                 |
| (¬P ∨ R) ∨ (¬Q ∨ R) | conditional law |
| (¬P ∨ R) ∨ (R ∨ ¬Q) | commutative law |
| ¬P ∨ (R ∨ R) ∨ ¬Q   | associative law |
| ¬P ∨ ¬Q ∨ R         | commutative law |
| ¬(P ∧ Q) ∨ R        | DeMorgan's law  |
| (P ∧ Q) → R         | conditional law |

Therefore (P → R) ∨ (Q → R) is equivalent to (P ∧ Q) → R.

** Exercise 7

*** 7a

(P → Q) ∧ (Q → R) is equivalent to (P → R) ∧ [(P ↔ Q) ∨ (R ↔ Q)].

Goal: (P → R) ∧ [(P ↔ Q) ∨ (R ↔ Q)]

Start from RHS:
| Step                                                        | Law used                         |
|-------------------------------------------------------------+----------------------------------|
| (P → R) ∧ [(P ↔ Q) ∨ (R ↔ Q)]                             |                                  |
| (P → R) ∧ [((P → Q) ∧ (Q → P)) ∨ ((R → Q) ∧ (Q → R))]     | biconditional defn.              |
| (P → R) ∧ [((¬P ∨ Q) ∧ (¬Q ∨ P)) ∨ ((¬R ∨ Q) ∧ (¬Q ∨ R))] | conditional law                  |
| (P → R) ∧ [((¬P ∧ ¬Q) ∨ (P ∧ Q)) ∨ ((¬R ∧ ¬Q) ∨ (R ∧ Q))] | contradiction law                |
| (P → R) ∧ [((P ∧ Q) ∨ (R ∧ Q)) ∨ ((¬P ∧ ¬Q) ∨ (¬R ∧ ¬Q))] | associative and commutative laws |
| (P → R) ∧ [((P ∨ R) ∧ Q) ∨ ((¬P ∨ ¬R) ∧ ¬Q)]              | distributive law                 |
| (¬P ∨ R) ∧ [((P ∨ R) ∧ Q) ∨ ((¬P ∨ ¬R) ∧ ¬Q)]             | conditional law                  |
| [(¬P ∨ R) ∧ (P ∨ R) ∧ Q] ∨ [(¬P ∨ R) ∧ (¬P ∨ ¬R) ∧ ¬Q]    | distributive law                 |
| [(R ∨ (¬P ∧ P)) ∧ Q] ∨ [(¬P ∨ (R ∧ ¬R)) ∧ ¬Q]             | distributive law                 |
| (R ∧ Q) ∨ (¬P ∧ ¬Q)                                       | contradiction law                |
| ((R ∧ Q) ∨ ¬P) ∧ ((R ∧ Q) ∨ ¬Q)                           | distributive law                 |
| ((R ∨ ¬P) ∧ (Q ∨ ¬P)) ∧ ((R ∨ ¬Q) ∧ (Q ∨ ¬Q))             | distributive law                 |
| ((R ∨ ¬P) ∧ (Q ∨ ¬P)) ∧ (R ∨ ¬Q)                          | tautology law                    |
| (R ∨ ¬P) ∧ (¬P ∨ Q) ∧ (¬Q ∨ R)                            | commutative and associative laws |
| (¬P ∨ Q) ∧ (¬Q ∨ R)                                       | can safely remove (R ∨ ¬P) term  |
| (P → Q) ∧ (Q → R)                                         | conditional law                  |


| P | Q | R | (R ∨ ¬P) | (¬P ∨ Q) | (¬Q ∨ R) | (R ∨ ¬P) ∧ (¬P ∨ Q) ∧ (¬Q ∨ R) | (¬P ∨ Q) ∧ (¬Q ∨ R) |
|---+---+---+----------+----------+----------+--------------------------------+---------------------|
| F | F | F | T        | T        | T        | T                              | T                   |
| F | F | T | T        | T        | T        | T                              | T                   |
| F | T | F | T        | T        | F        | F                              | F                   |
| F | T | T | T        | T        | T        | T                              | T                   |
| T | F | F | F        | F        | T        | F                              | F                   |
| T | F | T | T        | F        | T        | F                              | F                   |
| T | T | F | F        | T        | F        | F                              | F                   |
| T | T | T | T        | T        | T        | T                              | T                   |

Truth tables for (R ∨ ¬P) ∧ (¬P ∨ Q) ∧ (¬Q ∨ R) and (¬P ∨ Q) ∧ (¬Q ∨ R) are
equivalent therefore statements are equivalent.

Therefore (P → Q) ∧ (Q → R) is equivalent to (P → R) ∧ [(P ↔ Q) ∨ (R ↔ Q)].

*** 7b

| Step                 | Law used        |
|----------------------+-----------------|
| (P → Q) ∨ (Q → R)    |                 |
| (¬P ∨ Q) ∨ (¬Q ∨ R)  | conditional law |
| (¬P ∨ (Q ∨ ¬Q)) ∨ R  | associative law |
| (¬P ∨ tautology) ∨ R | tautology law   |
| tautology ∨ R        | tautology law   |
| tautology            | tautology law   |

Therefore (P → Q) ∨ (Q → R) is a tautology.

** Exercise 8

   P ∧ Q
   ¬(¬P ∨ ¬Q)
   ¬(P → ¬Q)

** Exercise 9
   P ↔ Q
   (P → Q) ∧ (Q → P)
   ¬(¬(P → Q) ∨ ¬(Q → P))
   ¬((P → Q) → (¬(Q → P)))

** Exercise 10

| P | Q | R | ¬P ∨ (¬Q ∨ R) | ¬Q ∨ (¬P ∨ R) | (¬P ∨ Q) ∧ (¬P ∨ R) | ¬(P ∧ Q) ∨ R | ¬P ∨ (Q ∧ R) |
|---+---+---+---------------+---------------+---------------------+--------------+--------------|
| F | F | F | T             | T             | T                   | T            | T            |
| F | F | T | T             | T             | T                   | T            | T            |
| F | T | F | T             | T             | T                   | T            | T            |
| F | T | T | T             | T             | T                   | T            | T            |
| T | F | F | T             | T             | F                   | T            | F            |
| T | F | T | T             | T             | F                   | T            | F            |
| T | T | F | F             | F             | F                   | F            | F            |
| T | T | T | T             | T             | T                   | T            | T            |

a, b and d are equivalent.
c and e are also equivalent.
