* Chapter 2.3 Exercise Solutions

** Exercise 1
- Analyze the logical forms of the following statements.

*** 1a
F ⊆ 𝒫(A)
F ⊆ {x \vert x ⊆ A }
∀x(x ∈ F → {x \vert x ⊆ A })
∀x(x ∈ F → ∀y(y ∈ x → y ∈ A))

*** 1b
A ⊆ {2n + 1 | n ∈ ℕ}
∀x(x ∈ A → x ∈ {2n + 1 | n ∈ ℕ})
∀x(x ∈ A → ∃n ∈ ℕ(x = 2n + 1))

*** 1c
{n^2 + n + 1 | n ∈ ℕ} ⊆ {2n + 1 | n ∈ ℕ}

∀x(x ∈ {n^2 + n + 1 | n ∈ ℕ} → x ∈ {2n + 1 | n ∈ ℕ})
∀x(∃n ∈ ℕ(x = n^2 + n + 1) → ∃m ∈ ℕ(x = 2m + 1))
∀n ∈ ℕ∃m ∈ ℕ(n^2 + n + 1 = 2m + 1)

*** 1d
𝒫(∪_{i∈I}A_i) ⊄ ∪_{i∈I}𝒫(A_i)
∃x(x ∈ 𝒫(∪_{i∈I}A_i) ∧ x ∉ ∪_{i∈I}𝒫(A_i))

x ∈ 𝒫(∪_{i∈I}A_i):
∀y(y ∈ x → y ∈ ∪_{i∈I}A_i)
∀y(y ∈ x → y ∈ {t \vert ∃i ∈ I(t ∈ A_i)})
∀y(y ∈ x → ∃i ∈ I(y ∈ A_i))

x ∉ ∪_{i∈I}𝒫(A_i):
x ∉ {t | ∃i ∈ I(t ∈ 𝒫(A_i))}
∃i ∈ I(x ∉ 𝒫(A_i))
∃i ∈ I(x ∉ {z | z ⊆ A_i })
∃i ∈ I(x ⊄ A_i)
∃i ∈ I∃y(y ∈ x ∧ y ∉ A_i)

∃x(x ∈ 𝒫(∪_{i∈I}A_i) ∧ x ∉ ∪_{i∈I}𝒫(A_i))
∃x(∀y(y ∈ x → ∃i ∈ I(y ∈ A_i)) ∧ ∃i ∈ I∃y(y ∈ x ∧ y ∉ A_i))

** Exercise 2
*** 2a
x ∈ ∪F \ ∪G
x ∈ ∪F ∧ x ∉ ∪G
∃A ∈ F(x ∈ A) ∧ ¬∃A ∈ G(x ∈ A)
∃A ∈ F(x ∈ A) ∧ ∀A ∈ G(x ∉ A)

*** 2b
{x ∈ B | x ∉ C} ∈ 𝒫(A)
{x ∈ B | x ∉ C} ∈ {x \vert x ⊆ A }
{x ∈ B | x ∉ C} ⊆ A
∀y(y ∈ {x ∈ B | x ∉ C} → y ∈ A)
∀y({y ∈ B | y ∉ C} → y ∈ A)
∀y(y ∈ B ∧ y ∉ C → y ∈ A)

*** 2c
x ∈ ∩_{i∈I}(A_i ∪ B_i)
x ∈ {x \vert ∀i ∈ I(x ∈ (A_i ∪ B_i))}
∀i ∈ I(x ∈ (A_i ∪ B_i))
∀i ∈ I(x ∈ A_i ∨ x ∈ B_i)

*** 2d
x ∈ (∩_{i∈I}A_i) ∪ (∩_{i∈I}B_i)
(∀i ∈ I(x ∈ A_i)) ∨ (∀i ∈ I(x ∈ B_i))

** Exercise 3
𝒫({∅}) = {∅, {∅}}
∅ is a subset of the set (it is of all sets).
{∅} is the subset containing the one element of the set.

** Exercise 4
∩F = {red, blue}
∪F = {red, green, blue, orange, purple}

** Exercise 5
∩F = ∅
∪F = {3, 7, 12, 5, 16, 23}

** Exercise 6
*** 6a
A_2 = {2,3,1,4}
A_3 = {3,4,2,6}
A_4 = {4,5,3,8}
A_5 = {5,6,4,10}

*** 6b
∩_{i∈I}A_i = {4}
∪_{i∈I}A_i = {1,2,3,4,5,6,8,10}

** Exercise 7
Ugh, really?

** Exercise 8
*** 8a
A_2 = {2,4}
A_3 = {3,6}

B_2 = {2,3}
B_3 = {3,4}

*** 8b
∩_{i∈I}(A_i ∪ B_i) = ∩{2,3,4}{3,4,6}
            = {3,4}

(∩_{i∈I}A_i) ∪ (∩_{i∈I}B_i) = {} ∪ {3}
                 = {3}

They are not the same.

*** 8c
From our answer in 8b, we can conclude that x ∈ ∩_{i∈I}(A_i ∪ B_i) and x ∈ (∩_{i∈I}A_i) ∪
(∩_{i∈I}B_i) are *not* equivalent statements.

** Exercise 9
I = {2, 3}
A_i = {i,2i}
B_i = {i,i+1}

A_2 = {2,4}
A_3 = {3,6}
B_2 = {2,3}
B_3 = {3,4}

∪_{i∈I}(A_i ∩ B_i)      = ∪{2}{3}             = {2,3}
(∪_{i∈I}A_i) ∩ (∪_{i∈I}B_i) = {2,3,4,6} ∩ {2,3,4} = {2,3,4}

** Exercise 10

x ∈ 𝒫(A ∩ B)
x ∈ {x \vert x ⊆ A ∩ B }
x ⊆ A ∩ B
∀y(y ∈ x → y ∈ A ∩ B)
∀y(y ∈ x → y ∈ A ∧ y ∈ B)
∀y(y ∉ x ∨ (y ∈ A ∧ y ∈ B)) [conditional law]
∀y((y ∉ x ∨ y ∈ A) ∧ (y ∉ x ∨ y ∈ B)) [distributive law]
∀y((y ∈ x → y ∈ A) ∧ (y ∈ x → y ∈ B)) [conditional law]

x ∈ 𝒫(A) ∩ 𝒫(B)
x ∈ {x \vert x ⊆ A } ∩ {x \vert x ⊆ B }
x ⊆ A ∧ x ⊆ B
∀y(y ∈ x → y ∈ A) ∧ ∀y(y ∈ x → y ∈ B)
∀y((y ∈ x → y ∈ A) ∧ (y ∈ x → y ∈ B)), which is equivalent to above.

** Exercise 11

A = {1,2}
B = {2,3}

𝒫(A ∪ B)    = 𝒫({1,2,3})
            = {∅, {1}, {2}, {3}, {1,2}, {1,3}, {2,3}}

𝒫(A) ∪ 𝒫(B) = {∅, {1}, {2}, {1,2}} ∪ {∅, {2}, {3}, {2,3}}
            = {∅, {1}, {2}, {3}, {1,2}, {2,3}}

** Exercise 12
*** 12a
∪_{i∈I}(A_i ∪ B_i):
x ∈ ∪_{i∈I}(A_i ∪ B_i)
x ∈ {x \vert ∃i ∈ I(x ∈ (A_i ∪ B_i))}
∃i ∈ I(x ∈ (A_i ∪ B_i))
∃i ∈ I(x ∈ A_i ∨ x ∈ B_i)

(∪_{i∈I}A_i) ∪ (∪_{i∈I}B_i):
x ∈ (∪_{i∈I}A_i) ∪ (∪_{i∈I}B_i)
x ∈ (∪_{i∈I}A_i) ∨ x ∈ (∪_{i∈I}B_i)
x ∈ {x \vert ∃i ∈ I(x ∈ A_i)} ∨ x ∈ {x \vert ∃i ∈ I(x ∈ B_i)}
∃i ∈ I(x ∈ A_i) ∨ ∃i ∈ I(x ∈ B_i)
∃i ∈ I(x ∈ A_i ∨ x ∈ B_i)

Therefore ∪_{i∈I}(A_i ∪ B_i) = (∪_{i∈I}A_i) ∪ (∪_{i∈I}B_i).

*** 12b
(∩F)∩(∩G) = ∩(F ∪ G)

(∩F)∩(∩G):
x ∈ (∩F)∩(∩G)
(x ∈ ∩F) ∧ (x ∈ ∩G)
x ∈ {x \vert ∀A ∈ F(x ∈ A)} ∧ x ∈ {x \vert ∀A ∈ G(x ∈ A)}
∀A ∈ F(x ∈ A) ∧ ∀A ∈ G(x ∈ A)

∩(F ∪ G):
x ∈ {x \vert ∀A ∈ (F ∪ G)(x ∈ A)}
∀A ∈ (F ∪ G)(x ∈ A)
∀A(A ∈ (F ∪ G) → x ∈ A)
∀A((A ∈ F ∨ A ∈ G) → x ∈ A)
∀A(¬(A ∈ F ∨ A ∈ G) ∨ x ∈ A)           [conditional law]
∀A((A ∉ F ∧ A ∉ G) ∨ x ∈ A)            [DeMorgan's law]
∀A((A ∉ F ∨ x ∈ A) ∧ (A ∉ G ∨ x ∈ A))  [distributive law]
∀A((A ∈ F → x ∈ A) ∧ (A ∈ G → x ∈ A))  [conditional law]
∀A(A ∈ F → x ∈ A) ∧ ∀A(A ∈ G → x ∈ A)  [∀ distributes over ∧]
∀A ∈ F(x ∈ A) ∧ ∀A ∈ G(x ∈ A)

Therefore (∩F)∩(∩G) = ∩(F ∪ G).

*** 12c
∩_{i∈I}(A_i \ B_i) = ∩_{i∈I}A_i \ ∪_{i∈I}B_i

∩_{i∈I}(A_i \ B_i):
x ∈ {x \vert ∀i ∈ I(x ∈ (A_i \ B_i))}
∀i ∈ I(x ∈ (A_i \ B_i))
∀i ∈ I(x ∈ A_i ∧ x ∉ B_i) [defn. of set difference]

∩_{i∈I}A_i \ ∪_{i∈I}B_i:
x ∈ ∩_{i∈I}A_i \ ∪_{i∈I}B_i
x ∈ ∩_{i∈I}A_i ∧ x ∉ ∪_{i∈I}B_i [defn. of set difference]
x ∈ {x \vert ∀i ∈ I(x ∈ A_i)} ∧ x ∉ {x \vert ∃i ∈ I(x ∈ B_i)}
∀i ∈ I(x ∈ A_i) ∧ ¬(∃i ∈ I(x ∈ B_i))
∀i ∈ I(x ∈ A_i) ∧ ∀i ∈ I(x ∉ B_i) [quantifier negation law]
∀i ∈ I(x ∈ A_i ∧ x ∉ B_i)

** Exercise 13
I = {1,2}
J = {3,4}
A_{i,j} = {i,j,i+j}

*** 13a
For each j ∈ J, let B_j = ∪_{i∈I}A_i,j = A_1,j ∪ A_2,j. Find B_3 and B_4.
B_3 = A_1,3 ∪ A_2,3
   = {1,3,4} ∪ {2,3,5}
   = {1,2,3,4,5}

B_4 = A_1,4 ∪ A_2,4
   = {1,4,5} ∪ {2,4,6}
   = {1,2,4,5,6}

*** 13b
∩_{j∈J}B_j = ∩_{j∈J}(∪_{i∈I}A_{i,j})
∩_{j∈J}(∪_{i∈I}A_{i,j})
∩_{j∈J}(A_{1,j} ∪ A_{2,j})
((A_{1,3} ∪ A_{2,3}) ∩ (A_{1,4} ∪ A_{2,4}))
(({1,3,4} ∪ {2,3,5}) ∩ ({1,4,5} ∪ {2,4,6}))
{1,2,3,4,5} ∩ {1,2,4,5,6}
{1,2,4,5}

*** 13c
∪_{i∈I}_{}_{}(∩_{j∈J}_{}A_{i,j})
∪_{i∈I}_{}_{}(A_{i,3} ∩ A_{i,4})
(A_{1,3} ∩ A_{1,4}) ∪ (A_{2,3} ∩ A_{2,4})
({1,3,4} ∩ {1,4,5}) ∪ ({2,3,5} ∩ {2,4,6})
{1,4} ∪ {2}
{1,2,4}

∪_{i∈I}_{}_{}(∩_{j∈J}_{}A_{i,j}) and ∩_{j∈J}(∪_{i∈I}A_{i,j}) are not equal.

*** 13d
∪_{i∈I}_{}_{}(∩_{j∈J}_{}A_{i,j}):
x ∈ ∪_{i∈I}_{}_{}(∩_{j∈J}_{}A_{i,j})
x ∈ {x \vert ∃i ∈ I(x ∈ (∩_{j∈J}_{}A_{i,j}))}
∃i ∈ I(x ∈ (∩_{j∈J}_{}A_{i,j}))
∃i ∈ I(x ∈ ({x \vert ∀j ∈ J(x ∈ A_{i,j})}))
∃i ∈ I(∀j ∈ J(x ∈ A_{i,j}))


∩_{j∈J}(∪_{i∈I}A_{i,j}):
x ∈ ∩_{j∈J}(∪_{i∈I}A_{i,j})
x ∈ {x \vert ∀j ∈ J(x ∈ (∪_{i∈I}A_{i,j}))}
∀j ∈ J(x ∈ (∪_{i∈I}A_{i,j}))
∀j ∈ J(∃i ∈ I(x ∈ A_{i,j}))

They are not equivalent.

** Exercise 14
*** 14a
x ∈ ∪F
x ∈ {x \vert ∃A ∈ F(x ∈ A)}
∃A ∈ F(x ∈ A)
∃A(A ∈ F ∧ x ∈ A)
∃A(A ∈ ∅ ∧ x ∈ A) [F = ∅]

A ∈ ∅ is always false and so (A ∈ ∅ ∧ x ∈ A) will always be false.

*** 14b
x ∈ ∩F
x ∈ {x \vert ∀A ∈ F(x ∈ A)}
∀A ∈ F(x ∈ A)
∀A(A ∈ F → x ∈ A)
∀A(A ∉ F ∨ x ∈ A) [conditional equivalence]
∀A(A ∉ ∅ ∨ x ∈ A) [F = ∅]

A ∉ ∅ is always true so (A ∉ ∅ ∨ x ∈ A) will also always be true.

** Exercise 15
*** 15a
Let R be all sets that are not elements of themselves.
R = {A ∈ U | A ∉ A}
∀A ∈ U(A ∈ R ↔ A ∉ A)
R ∈ ∀A ∈ U(A ∈ R ↔ A ∉ A)
(R ∈ R ↔ R ∉ R)
(T ↔ F)
(T → F) ∧ (F → T) [biconditional equivalence]
(F ∨ F) ∧ (T ∨ T) [conditional equivalence]
F ∧ T
F [contradiction]

*** 15b
A universal set of sets does not exist, the universal set can't contain itself.
