* Chapter 3.2 Exercise Solutions

** Exercise 1
*** 1a
Suppose P → Q and Q → R are both true. Prove that P → R is true.

| Givens | Goals |
|--------+-------|
| P → Q  | P → R |
| Q → R  |       |

| Givens | Goals |
|--------+-------|
| P → Q  | R     |
| Q → R  |       |
| P      |       |

Suppose P.
  [Proof of R goes here.]
Therefore P → R.

| Givens | Goals |
|--------+-------|
| P → Q  | R     |
| Q → R  |       |
| P      |       |
| Q      |       |

Suppose P.
  Since P and P → Q, it follows that Q is true.
  [Proof of R goes here.]
Therefore P → R.

/Solution/
*Theorem:* /Suppose P → Q and Q → R are both true. Then P → R is true./
Suppose P. Since P and P → Q, it follows that Q. But since Q and Q → R, we can
conclude R. Therefore P → R.

*** 1b
Suppose ¬R → (P → ¬Q) is true. Prove that P → (Q → R) is true.

| Givens        | Goals       |
|---------------+-------------|
| ¬R → (P → ¬Q) | P → (Q → R) |

| Givens        | Goals |
|---------------+-------|
| ¬R → (P → ¬Q) | Q → R |
| P             |       |

Suppose P.
  [Proof of Q → R goes here.]
Therefore P → (Q → R).

Prove contrapositive:
| Givens        | Goals |
|---------------+-------|
| ¬R → (P → ¬Q) | ¬Q    |
| P             |       |
| ¬R            |       |

Suppose P.
  Prove contrapositive: ¬R → ¬Q.
  Suppose ¬R.
    [Proof of ¬Q goes here.]
  Therefore ¬R → ¬Q
Therefore P → (Q → R).

| Givens        | Goals |
|---------------+-------|
| ¬R → (P → ¬Q) | ¬Q    |
| P             |       |
| ¬R            |       |
| P → ¬Q        |       |

| Givens        | Goals |
|---------------+-------|
| ¬R → (P → ¬Q) | ¬Q    |
| P             |       |
| ¬R            |       |
| P → ¬Q        |       |
| ¬Q            |       |

Suppose P.
  Prove contrapositive: ¬R → ¬Q.
  Suppose ¬R.
    We are given ¬R → (P → ¬Q), so can conclude P → ¬Q. We are also given P and so can conclude ¬Q.
  Therefore ¬R → ¬Q
Therefore P → (Q → R).

/Solution/
*Theorem:* /Suppose ¬R → (P → ¬Q) is true. Then P → (Q → R) is also true./
Suppose P. We will prove the contrapositive of Q → R: ¬R → ¬Q. Suppose ¬R. We
are given ¬R → (P → ¬Q), so can conclude P → ¬Q. We are also given P and so can
conclude ¬Q. Therefore ¬R → ¬Q and so Q → R. Thus, we can conclude that if ¬R →
(P → ¬Q) is true, then P → (Q → R) is also true.

** Exercise 2
*** 2a
Suppose P → Q and R → ¬Q are both true. Prove that P → ¬R is true.

| Givens | Goals  |
|--------+--------|
| P → Q  | P → ¬R |
| R → ¬Q |        |


| Givens | Goals |
|--------+-------|
| P → Q  | ¬R    |
| R → ¬Q |       |
| P      |       |

Suppose P.
  [Proof of ¬R.]
Therefore P → ¬R.

| Givens | Goals |
|--------+-------|
| P → Q  | ¬R    |
| R → ¬Q |       |
| P      |       |
| Q → ¬R |       |

Suppose P.
  Given R → ¬Q, by contrapositive law, also given Q → ¬R.
  [Proof of ¬R.]
Therefore P → ¬R.

| Givens | Goals |
|--------+-------|
| P → Q  | ¬R    |
| R → ¬Q |       |
| P      |       |
| Q → ¬R |       |
| Q      |       |

Suppose P.
  Given R → ¬Q, by contrapositive law, also given Q → ¬R.
  Given P → Q and P, thus can conclude Q.
  [Proof of ¬R.]
Therefore P → ¬R.

| Givens | Goals |
|--------+-------|
| P → Q  | ¬R    |
| R → ¬Q |       |
| P      |       |
| Q → ¬R |       |
| Q      |       |
| ¬R     |       |

Suppose P.
  Given R → ¬Q, by contrapositive law, also given Q → ¬R.
  Given P → Q and P, thus can conclude Q.
  Given Q → ¬R and Q, thus can conclude ¬R.
Therefore P → ¬R.

/Solution/
*Theorem:* /Suppose P → Q and R → ¬Q are both true. Then P → ¬R is true./
Suppose P. Given R → ¬Q, by the contrapositive law, we also know Q → ¬R. Given P
→ Q and P, we can conclude Q. Given Q → ¬R and Q, we can conclude ¬R. Therefore
if P → Q and R → ¬Q and true, P → ¬R is true.

*** 2b

Suppose that P is true. Prove that Q → ¬(Q → ¬P) is true.

| Givens | Goals         |
|--------+---------------|
| P      | Q → ¬(Q → ¬P) |

| Givens | Goals     |
|--------+-----------|
| P      | ¬(Q → ¬P) |
| Q      |           |

Suppose Q.
  [Proof of ¬(Q → ¬P) goes here.]
Therefore Q → ¬(Q → ¬P).

| Givens | Goals      |
|--------+------------|
| P      | ¬(¬Q ∨ ¬P) |
| Q      |            |

| Givens | Goals |
|--------+-------|
| P      | Q ∧ P |
| Q      |       |

Suppose Q.
  ¬(Q → ¬P) is the same as Q ∧ P.
  [Proof of Q ∧ P goes here.]
Therefore Q → ¬(Q → ¬P).

Suppose Q.
  ¬(Q → ¬P) is the same as Q ∧ P.
  Given both Q and P, thus can conclude Q ∧ P.
Therefore Q → ¬(Q → ¬P).

/Solution/
*Theorem:* /Suppose P is true. Then Q → ¬(Q → ¬P) is true./
Suppose Q. ¬(Q → ¬P) is the same as Q ∧ P. We are given both Q and P, thus can
conclude Q ∧ P. Therefore if P is true, Q → ¬(Q → ¬P) is true.

** Exercise 3
Suppose A ⊆ C, and B and C are disjoint. Prove that if x ∈ A then x ∉ B.

| Givens    | Goals         |
|-----------+---------------|
| A ⊆ C     | x ∈ A → x ∉ B |
| B ∩ C = ∅ |               |

| Givens            | Goals         |
|-------------------+---------------|
| ∀x(x ∈ A → x ∈ C) | x ∈ A → x ∉ B |
| ∀x(x ∈ B → x ∉ C) |               |

A ⊆ C is the same as saying ∀x(x ∈ A → x ∈ C) and "B and C are disjoint" is the
same as saying ∀x(x ∈ B → x ∉ C).

| Givens            | Goals |
|-------------------+-------|
| ∀x(x ∈ A → x ∈ C) | x ∉ B |
| ∀x(x ∈ B → x ∉ C) |       |
| x ∈ A             |       |

A ⊆ C is the same as saying ∀x(x ∈ A → x ∈ C) and "B and C are disjoint" is the
same as saying ∀x(x ∈ B → x ∉ C).
Suppose x ∈ A.
  [Proof of x ∉ B.]
Therefore x ∈ A → x ∉ B.

| Givens            | Goals |
|-------------------+-------|
| ∀x(x ∈ A → x ∈ C) | x ∉ B |
| ∀x(x ∈ B → x ∉ C) |       |
| x ∈ A             |       |
| x ∈ C             |       |

A ⊆ C is the same as saying ∀x(x ∈ A → x ∈ C) and "B and C are disjoint" is the
same as saying ∀x(x ∈ B → x ∉ C).
Suppose x ∈ A.
  From ∀x(x ∈ A → x ∈ C) we can conclude x ∈ C.
  [Proof of x ∉ B.]
Therefore x ∈ A → x ∉ B.

| Givens            | Goals |
|-------------------+-------|
| ∀x(x ∈ A → x ∈ C) | x ∉ B |
| ∀x(x ∈ B → x ∉ C) |       |
| x ∈ A             |       |
| x ∈ C             |       |
| ∀x(x ∈ C → x ∉ B) |       |

A ⊆ C is the same as saying ∀x(x ∈ A → x ∈ C) and "B and C are disjoint" is the
same as saying ∀x(x ∈ B → x ∉ C).
Suppose x ∈ A.
  From ∀x(x ∈ A → x ∈ C) we can conclude x ∈ C.
  By contrapositive law, ∀x(x ∈ B → x ∉ C) is same as ∀x(x ∈ C → x ∉ B).
  [Proof of x ∉ B.]
Therefore x ∈ A → x ∉ B.

| Givens            | Goals |
|-------------------+-------|
| ∀x(x ∈ A → x ∈ C) | x ∉ B |
| ∀x(x ∈ B → x ∉ C) |       |
| x ∈ A             |       |
| x ∈ C             |       |
| ∀x(x ∈ C → x ∉ B) |       |
| x ∉ B             |       |

A ⊆ C is the same as saying ∀x(x ∈ A → x ∈ C) and "B and C are disjoint" is the
same as saying ∀x(x ∈ B → x ∉ C).
Suppose x ∈ A.
  From ∀x(x ∈ A → x ∈ C) we can conclude x ∈ C.
  By contrapositive law, ∀x(x ∈ B → x ∉ C) is same as ∀x(x ∈ C → x ∉ B).
  Given ∀x(x ∈ C → x ∉ B) and assumed x ∈ C, thus can conclude x ∉ B.
Therefore x ∈ A → x ∉ B.

/Solution/
*Theorem:* /Suppose A ⊆ C, and B and C are disjoint. If x ∈ A then x ∉ B./ A ⊆ C
is the same as saying ∀x(x ∈ A → x ∈ C) and "B and C are disjoint" is the same
as saying ∀x(x ∈ B → x ∉ C). Suppose x ∈ A. From ∀x(x ∈ A → x ∈ C) we can
conclude x ∈ C. By contrapositive law, ∀x(x ∈ B → x ∉ C) is same as ∀x(x ∈ C → x
∉ B). We are given ∀x(x ∈ C → x ∉ B) and we assumed x ∈ C, thus can conclude
x ∉ B. Therefore if A ⊆ C, and B and C are disjoint, then if x ∈ A then x ∉ B.

** Exercise 4
Suppose that A \ B is disjoint from C and x ∈ A. Prove that if x ∈ C then x ∈ B.

| Givens                   | Goals         |
|--------------------------+---------------|
| A \ B is disjoint from C | x ∈ C → x ∈ B |
| x ∈ A                    |               |

| Givens                   | Goals         |
|--------------------------+---------------|
| A \ B is disjoint from C | x ∈ C → x ∈ B |
| x ∈ A                    |               |

A \ B is disjoint from C is the same as saying ∀x(x ∈ A \ B → x ∉ C) or
∀x(x ∈ A ∧ x ∉ B → x ∉ C)
∀x(¬(x ∈ A ∧ x ∉ B) ∨ x ∉ C)
∀x(x ∉ A ∨ x ∈ B ∨ x ∉ C)

A \ B is disjoint from C is the same as saying ∀x(x ∉ A ∨ x ∈ B ∨ x ∉ C)

| Givens                | Goals         |
|-----------------------+---------------|
| x ∉ A ∨ x ∈ B ∨ x ∉ C | x ∈ C → x ∈ B |
| x ∈ A                 |               |

A \ B is disjoint from C is the same as saying ∀x(x ∉ A ∨ x ∈ B ∨ x ∉ C)

| Givens                | Goals |
|-----------------------+-------|
| x ∉ A ∨ x ∈ B ∨ x ∉ C | x ∈ B |
| x ∈ A                 |       |
| x ∈ C                 |       |

A \ B is disjoint from C is the same as saying ∀x(x ∉ A ∨ x ∈ B ∨ x ∉ C)
Suppose x ∈ C
  [Proof of x ∈ B.]
Therefore x ∈ C → x ∈ B.

A \ B is disjoint from C is the same as saying ∀x(x ∉ A ∨ x ∈ B ∨ x ∉ C)
Suppose x ∈ C.
  Given x ∉ A ∨ x ∈ B ∨ x ∉ C is true and know x ∈ A and x ∈ C, thus can conclude that x ∈ B.
Therefore x ∈ C → x ∈ B.

/Solution/
*Theorem:* Suppose that A \ B is disjoint from C and x ∈ A. If x ∈ C then x ∈ B.
/Proof./ A \ B is disjoint from C is the same as saying
∀x(x ∉ A ∨ x ∈ B ∨ x ∉ C) Suppose x ∈ C. Given x ∉ A ∨ x ∈ B ∨ x ∉ C is true and
know x ∈ A and x ∈ C, thus we can conclude that x ∈ B. Therefore x ∈ C → x ∈ B.

** Exercise 5
Use the method of proof by contradiction to prove: "Suppose A ∩ C ⊆ B and a ∈ C.
Prove that a ∉ A \ B."

| Givens    | Goals     |
|-----------+-----------|
| A ∩ C ⊆ B | a ∉ A \ B |
| a ∈ C     |           |

| Givens    | Goals         |
|-----------+---------------|
| A ∩ C ⊆ B | Contradiction |
| a ∈ C     |               |
| a ∈ A \ B |               |

Suppose a ∈ A \ B.
  [Proof of contradiction.]
Therefore a ∉ A \ B.

| Givens        | Goals         |
|---------------+---------------|
| A ∩ C ⊆ B     | Contradiction |
| a ∈ C         |               |
| a ∈ A ∧ a ∉ B |               |

Suppose a ∈ A \ B.
  a ∈ A \ B is the same as saying a ∈ A ∧ a ∉ B.
  [Proof of contradiction.]
Therefore a ∉ A \ B.

| Givens    | Goals         |
|-----------+---------------|
| A ∩ C ⊆ B | Contradiction |
| a ∈ C     |               |
| a ∈ A     |               |
| a ∉ B     |               |

| Givens                    | Goals         |
|---------------------------+---------------|
| ∀x(x ∈ A ∧ x ∈ C → x ∈ B) | Contradiction |
| a ∈ C                     |               |
| a ∈ A                     |               |
| a ∉ B                     |               |

Suppose a ∈ A \ B.
  a ∈ A \ B is the same as saying a ∈ A ∧ a ∉ B.
  A ∩ C ⊆ B is the same as saying ∀x(x ∈ A ∧ x ∈ C → x ∈ B).
    Given a ∈ A ∧ a ∈ C → a ∈ B and a ∈ C. Supposed a ∈ A. Thus we conclude a ∈ B. But this contradicts our a ∉ B supposition.
Therefore a ∉ A \ B.

/Solution/
*Theorem:* Suppose A ∩ C ⊆ B and a ∈ C. Then a ∉ A \ B.
/Proof./ A ∩ C ⊆ B is the same as saying ∀x(x ∈ A ∧ x ∈ C → x ∈ B). Suppose
a ∈ A \ B. a ∈ A \ B is the same as saying a ∈ A ∧ a ∉ B.
Given a ∈ A ∧ a ∈ C → a ∈ B and a ∈ C. Supposed a ∈ A. Thus we conclude a ∈ B.
But this contradicts our a ∉ B supposition. Therefore a ∉ A \ B.

** Exercise 6
Use the method of proof by contradiction to prove: "Suppose that A ⊆ B, a ∈ A,
and a ∉ B \ C. Then a ∈ C."

| Givens    | Goals |
|-----------+-------|
| A ⊆ B     | a ∈ C |
| a ∈ A     |       |
| a ∉ B \ C |       |


| Givens            | Goals |
|-------------------+-------|
| ∀x(x ∈ A → x ∈ B) | a ∈ C |
| a ∈ A             |       |
| ¬(a ∈ B \ C)      |       |

A ⊆ B is the same as saying ∀x(x ∈ A → x ∈ B).

| Givens        | Goals |
|---------------+-------|
| a ∈ A → a ∈ B | a ∈ C |
| a ∈ A         |       |
| a ∉ B ∨ a ∈ C |       |

A ⊆ B is the same as saying ∀x(x ∈ A → x ∈ B).
a ∉ B \ C is the same as saying a ∉ B ∨ a ∈ C.

| Givens        | Goals         |
|---------------+---------------|
| a ∈ A → a ∈ B | Contradiction |
| a ∈ A         |               |
| a ∈ B → a ∈ C |               |
| a ∉ C         |               |

A ⊆ B is the same as saying ∀x(x ∈ A → x ∈ B).
a ∉ B \ C is the same as saying a ∈ B → a ∈ C.
Suppose a ∉ C.
  [Proof of contradiction.]
Therefore a ∈ C.

| Givens        | Goals         |
|---------------+---------------|
| a ∈ A → a ∈ B | Contradiction |
| a ∈ A         |               |
| a ∈ B → a ∈ C |               |
| a ∉ C         |               |
| a ∈ B         |               |

A ⊆ B is the same as saying ∀x(x ∈ A → x ∈ B).
a ∉ B \ C is the same as saying a ∉ B ∨ a ∈ C.
Suppose a ∉ C.
  We are given a ∈ A → a ∈ B and a ∈ A, thus we can conclude a ∈ B.
  We are given a ∈ B → a ∈ C and we know a ∈ B and thus we can conclude that a ∈ C.
  However, this contradicts our supposition that a ∉ C.
Therefore a ∈ C.

/Solution/
*Theorem:* /Suppose that A ⊆ B, a ∈ A, and a ∉ B \ C. Then a ∈ C./
/Proof./ A ⊆ B is the same as saying ∀x(x ∈ A → x ∈ B). a ∉ B \ C is the same as
saying a ∉ B ∨ a ∈ C. Suppose a ∉ C. We are given a ∈ A → a ∈ B and a ∈ A, thus
we can conclude a ∈ B. We are given a ∈ B → a ∈ C and we know a ∈ B and thus we
can conclude that a ∈ C. However, this contradicts our supposition that a ∉ C.
Therefore a ∈ C.

** Exercise 7
Suppose that y + x = 2y - x, and x and y are not both zero. Prove that y ≠ 0.

| Givens                    | Goals |
|---------------------------+-------|
| y + x = 2y - x            | y ≠ 0 |
| x and y are not both zero |       |

y + x = 2y - x
y - 2x = 0
y = 2x

y + x = 2y - x is the same as saying y = 2x.

| Givens                    | Goals         |
|---------------------------+---------------|
| y = 2x                    | Contradiction |
| x and y are not both zero |               |
| y = 0                     |               |

y + x = 2y - x is the same as saying y = 2x.
Suppose y = 0.
  [Proof of contradiction here.]
Therefore y ≠ 0.

| Givens                    | Goals         |
|---------------------------+---------------|
| y = 2x                    | Contradiction |
| x and y are not both zero |               |
| y = 0                     |               |
| x = 0                     |               |

y + x = 2y - x is the same as saying y = 2x.
Suppose y = 0.
  By y = 2x, can conclude that x = 0. But this contradicts our given that x and y are not both zero.
Therefore y ≠ 0.

/Solution/
*Theorem:* /Suppose that y + x = 2y - x, and x and y are not both zero. Prove that y ≠ 0./
/Proof./ y + x = 2y - x is the same as saying y = 2x. Suppose y = 0. By y = 2x,
we can conclude that x = 0. But this contradicts our given that x and y are not
both zero. Therefore y ≠ 0.

** Exercise 8
Suppose that a and b are nonzero real numbers. Prove that if a < 1/a < b < 1/b
then a < -1.

| Givens | Goals                      |
|--------+----------------------------|
| a ≠ 0  | a < 1/a < b < 1/b → a < -1 |
| b ≠ 0  |                            |
| a ∈ ℝ  |                            |
| b ∈ ℝ  |                            |

| Givens            | Goals  |
|-------------------+--------|
| a ≠ 0             | a < -1 |
| b ≠ 0             |        |
| a ∈ ℝ             |        |
| b ∈ ℝ             |        |
| a < 1/a < b < 1/b |        |

Suppose that a < 1/a < b < 1/b.
  [Proof of a < -1.]
Therefore if a < 1/a < b < 1/b, then a < -1.

1/a < 1/b
b < a [Multiply both sides by ab]
a > b
But given a < b, therefore ab is a negative number.

| Givens            | Goals  |
|-------------------+--------|
| a ≠ 0             | a < -1 |
| b ≠ 0             |        |
| a ∈ ℝ             |        |
| b ∈ ℝ             |        |
| a < 1/a < b < 1/b |        |
| ab < 0            |        |

Suppose that a < 1/a < b < 1/b.
  Multiplying both sides of the inequalty 1/a < 1/b by ab, we get a > b.
  However, we were given a < b, therefore ab must be a negative number.
  a < b and ab < 0 therefore a < 0.
  a < 0 and a ≠ 0, thus a < -1.
Therefore if a < 1/a < b < 1/b, then a < -1.

/Solution/
*Theorem:* /Suppose that a and b are nonzero real numbers. Prove that if a < 1/a
< b < 1/b then a < -1./
/Proof./ Suppose that a < 1/a < b < 1/b. Multiplying both sides of the inequalty
1/a < 1/b by ab, we get a > b. However, we were given a < b, therefore ab must
be a negative number. a < b and ab < 0 therefore a < 0. a < 0 and a ≠ 0, thus
a < -1. Therefore if a < 1/a < b < 1/b, then a < -1.

** Exercise 9
Suppose that x and y are real numbers. Prove that if x^{2}y = 2x + y, then if y ≠ 0
then x ≠ 0.

| Givens                   | Goals         |
|--------------------------+---------------|
| x and y are real numbers | y ≠ 0 → x ≠ 0 |
| x^{2}y = 2x + y             |               |


| Givens                   | Goals |
|--------------------------+-------|
| x and y are real numbers | x ≠ 0 |
| x^{2}y = 2x + y             |       |
| y ≠ 0                    |       |

Suppose y ≠ 0.
  [Proof of x ≠ 0]
Therefore if y ≠ 0, then x ≠ 0.

| Givens                   | Goals         |
|--------------------------+---------------|
| x and y are real numbers | Contradiction |
| x^{2}y = 2x + y             |               |
| y ≠ 0                    |               |
| x = 0                    |               |

Suppose y ≠ 0.
  Suppose x = 0.
    From x = 0 and x^{2}y = 2x + y we can conclude that y = 0. But this contradicts
    our earlier supposition that y ≠ 0.
  Therefore x ≠ 0.
Therefore if y ≠ 0, then x ≠ 0.

If x = 0:
  x^{2}y = 2x + y             
  0^{}y = 0 + y             
  y = 0

/Solution/
*Theorem:* /Suppose that x and y are real numbers. If x^{2}y = 2x + y, then if 
y ≠ 0 then x ≠ 0./
/Proof./ Suppose y ≠ 0. Suppose x = 0. From x = 0 and x^{2}y = 2x + y we can
conclude that y = 0. But this contradicts our earlier supposition that y ≠ 0.
Therefore x ≠ 0. Thus if y ≠ 0, then x ≠ 0. Therefore, if x and y are real
numbers and if x^{2}y = 2x + y, then if y ≠ 0, then x ≠ 0.

** Exercise 10
Suppose that x and y are real numbers. Prove that if x ≠ 0, then if 
y = (3x^{2} + 2y)/(x^2 + 2) then y = 3.

| Givens                   | Goals                           |
|--------------------------+---------------------------------|
| x and y are real numbers | y = (3x^{2} + 2y)/(x^2 + 2) → y = 3 |
| x ≠ 0                    |                                 |

| Givens                   | Goals |
|--------------------------+-------|
| x and y are real numbers | y = 3 |
| x ≠ 0                    |       |
| y = (3x^{2} + 2y)/(x^2 + 2)  |       |

Suppose y = (3x^{2} + 2y)/(x^2 + 2).
  Solving y = (3x^{2} + 2y)/(x^2 + 2), we get y = 3.
Therefore if y = (3x^{2} + 2y)/(x^2 + 2) → y = 3.

y = (3x^{2} + 2y)/(x^2 + 2)  
=> y(x^2 + 2) = 3x^2 + 2y
=> x^{2}y + 2y = 3x^2 + 2y
=> x^{2}y = 3x^2
=> y = 3

/Solution/
*Theorem:* /Suppose that x and y are real numbers. Prove that if x ≠ 0, then if
y = (3x^{2} + 2y)/(x^2 + 2) then y = 3./
/Proof./ Suppose y = (3x^{2} + 2y)/(x^2 + 2). Solving y = (3x^{2} + 2y)/(x^2 + 2), we
get y = 3. Thus if y = (3x^{2} + 2y)/(x^2 + 2) then y = 3. Therefore if x ≠ 0, then
if y = (3x^{2} + 2y)/(x^2 + 2) then y = 3.

** Exercise 11
*** 11a
The conclusion of the theorem can be expressed as: x ≠ 3 ∧ y ≠ 8.
If the conclusion is false, this can be expressed as: ¬(x ≠ 3 ∧ y ≠ 8). Which
simplifies to x = 3 ∨ y = 8. The problem with the proof is that it states that
if the conclusion of the theorem is false, then x = 3 and y = 8. This is
incorrect. As shown above, if the conclusion of the theorem is false
x = 3 or y = 8.

*** 11b
A counter-example to this theorem is: x = 3, y = 7.

** Exercise 12
*** 12a
(x ∉ B) ∧ (B ⊆ C) does not imply x ∉ C. Any x that is an element of C \ B is an
example. They are not an element of B and still an element of C.

A ⊆ C = ∀x(x ∈ A → x ∈ C)
B ⊆ C = ∀x(x ∈ B → x ∈ C)
If x ∈ A, x ∈ C.
x ∈ B → x ∈ C is given, but x ∉ B → x ∉ C is not given. By the given, if x ∈ B
is false, x ∈ C could be either true or false (anything follows from falsehood).
So we cannot conclude x ∉ C from x ∉ B.

*** 12b
Any element of A \ B is a counter-example to this theorem.

C = {1, 2, 3, 4, 5}, A = {1, 2, 3}, B = {3, 4, 5}, x = 1

** Exercise 13
Use truth tables to show that modus tollens is a valid rule of inference.

| P | Q | P → Q |
|---+---+-------|
| F | F | T     |
| F | T | T     |
| T | F | F     |
| T | T | T     |

/Modus Tollens:/ If you know that P → Q is true and Q is false, you can conclude
that P is false.

Every time P → Q is true and Q is false, P is false. Therefore modus tollens is
a valid rule of inference.

** Exercise 14

Suppose P → (Q → R). Prove that ¬R → (P → ¬Q).

| P | Q | R | P → ¬Q | Q → R | P → (Q → R) | ¬R → (P → ¬Q) | [P → (Q → R)] → [¬R → (P → ¬Q)] |
|---+---+---+--------+-------+-------------+---------------+---------------------------------|
| F | F | F | T      | T     | T           | T             | T                               |
| F | F | T | T      | T     | T           | T             | T                               |
| F | T | F | T      | F     | T           | T             | T                               |
| F | T | T | T      | T     | T           | T             | T                               |
| T | F | F | T      | T     | T           | T             | T                               |
| T | F | T | T      | T     | T           | T             | T                               |
| T | T | F | F      | F     | F           | F             | T                               |
| T | T | T | F      | T     | T           | T             | T                               |

** Exercise 15
*** 15a

| P | Q | R | P → Q | Q → R | P → R |
|---+---+---+-------+-------+-------|
| F | F | F | T     | T     | T     |
| F | F | T | T     | T     | T     |
| F | T | F | T     | F     | T     |
| F | T | T | T     | T     | T     |
| T | F | F | F     | T     | F     |
| T | F | T | F     | T     | T     |
| T | T | F | T     | F     | F     |
| T | T | T | T     | T     | T     |

P → R is true every time (P → Q) ∧ (Q → R) is true.

*** 15b
| P | Q | R | P → ¬Q | Q → R | ¬R → (P → ¬Q) | P → (Q → R) | [¬R → (P → ¬Q)] → [P → (Q → R)] |
|---+---+---+--------+-------+---------------+-------------+---------------------------------|
| F | F | F | T      | T     | T             | T           | T                               |
| F | F | T | T      | T     | T             | T           | T                               |
| F | T | F | T      | F     | T             | T           | T                               |
| F | T | T | T      | T     | T             | T           | T                               |
| T | F | F | T      | T     | T             | T           | T                               |
| T | F | T | T      | T     | T             | T           | T                               |
| T | T | F | F      | F     | F             | F           | T                               |
| T | T | T | F      | T     | T             | T           | T                               |

[¬R → (P → ¬Q)] → [P → (Q → R)] is always true. Therefore P → (Q → R) is true
whenever ¬R → (P → ¬Q) is true.

** Exercise 16
*** 16a
| P | R | Q | P → ¬Q | R → ¬Q | P → ¬R |
|---+---+---+--------+--------+--------|
| F | F | F | T      | T      | T      |
| F | T | F | T      | F      | T      |
| F | F | T | T      | T      | T      |
| F | T | T | T      | T      | T      |
| T | F | F | T      | T      | T      |
| T | T | F | T      | F      | F      |
| T | F | T | F      | T      | T      |
| T | T | T | F      | T      | F      |

P → ¬R is true whenever (P → ¬Q) ∧ (R → ¬Q) is true.

*** 16b

| P | Q | ¬(Q → ¬P) | Q → ¬(Q → ¬P) | P → [Q → ¬(Q → ¬P)] |
|---+---+-----------+---------------+---------------------|
| F | F | F         | T             | T                   |
| F | F | F         | T             | T                   |
| F | T | F         | F             | T                   |
| F | T | F         | F             | T                   |
| T | F | F         | T             | T                   |
| T | F | F         | T             | T                   |
| T | T | T         | T             | T                   |
| T | T | T         | T             | T                   |

P → [Q → ¬(Q → ¬P)] is always true.

** Exercise 17
Can the proof in Example 3.2.2 be modified to prove that if x^2 + y = 13 and 
x ≠ 3 then y ≠ 4? Explain.

| Givens      | Goals |
|-------------+-------|
| x^2 + y = 13 | y ≠ 4 |
| x ≠ 3       |       |


| Givens      | Goals         |
|-------------+---------------|
| x^2 + y = 13 | Contradiction |
| x ≠ 3       |               |
| y = 4       |               |

Suppose x^2 + y = 13 and x ≠ 3.
  Suppose y = 4.
    [Proof of contradiction.]
  Thus y ≠ 4.
Thus, if x^2 + y = 13 and x ≠ 3 then y ≠ 4.

x^2 + 4 = 13
x^2 = 9
x = ±3

It is not possible to modify the proof in Example 3.2.2 to prove y ≠ 4 because
if x = -3, y may equal 4. If we knew that these were natural numbers, we could
prove y ≠ 4.
