* Chapter 1.2 Exercise Solutions

** Exercise 1
*** 1a

| P | Q | (¬P ∨ Q) |
|---+---+----------|
| F | F | T        |
| F | T | T        |
| T | F | F        |
| T | T | T        |

*** 1b

| S | G | (S ∨ G) ∧ (¬S ∨ ¬G) |
|---+---+---------------------|
| F | F | F                   |
| F | T | T                   |
| T | F | T                   |
| T | T | F                   |

** Exercise 2
*** 2a

| P | Q | ¬[P ∧ (Q ∨ ¬P)] |
|---+---+-----------------|
| F | F | T               |
| F | T | T               |
| T | F | T               |
| T | T | F               |

*** 2b

| P | Q | R | (P ∨ Q) ∧ (¬P ∨ R) |
|---+---+---+--------------------|
| F | F | F | F                  |
| F | F | T | F                  |
| F | T | F | T                  |
| F | T | T | T                  |
| T | F | F | F                  |
| T | F | T | T                  |
| T | T | F | F                  |
| T | T | T | T                  |

** Exercise 3
*** 3a

| P | Q | P + Q |
|---+---+-------|
| F | F | F     |
| F | T | T     |
| T | F | T     |
| T | T | F     |

*** 3b

| P | Q | (P ∨ Q) ∧ (P ∨ Q) |
|---+---+-------------------|
| F | F | F                 |
| F | T | T                 |
| T | F | T                 |
| T | T | F                 |

** Exercise 4

¬(¬P ∧ ¬Q)

| P | Q | (P ∨ Q) | ¬(¬P ∧ ¬Q) |
|---+---+---------+------------|
| F | F | F       | F          |
| F | T | T       | T          |
| T | F | T       | T          |
| T | T | T       | T          |

** Exercise 5

*** 5a

| P | Q | P ↓ Q |
|---+---+-------|
| F | F | T     |
| F | T | F     |
| T | F | F     |
| T | T | F     |

*** 5b
¬P ∧ ¬Q

*** 5c
- ¬P is equivalent to P ↓ P
- P ∨ Q is equivalent to (P ↓ Q) ↓ (P ↓ Q)
- P ∧ Q is equivalent to (P ↓ P) ↓ (Q ↓ Q)

** Exercise 6

*** 6a

| P | Q | P \vert Q |
|---+---+-----------|
| F | F | T         |
| F | T | T         |
| T | F | T         |
| T | T | F         |

*** 6b

- ¬(P ∧ Q) is equivalent to P | Q

*** 6c

- ¬P is equivalent to P | P
- P ∨ Q is equivalent to (P | P) | (Q | Q)
- P ∧ Q is equivalent to (P | Q) | (P | Q)

** Exercise 7

Let P = Pete will win the math prize
    J = Jame will win the math prize
    C = Pete will win the chemistry prize

| P | J | C | ¬(P ∧ J) | (P ∨ C) | J | C |
|---+---+---+----------+---------+---+---|
| F | F | F | T        | F       | F | F |
| F | F | T | T        | T       | F | T |
| F | T | F | T        | F       | T | F |
| F | T | T | T        | T       | T | T |
| T | F | F | T        | T       | F | F |
| T | F | T | T        | T       | F | T |
| T | T | F | F        | T       | T | F |
| T | T | T | F        | T       | T | T |

C is true whenever all premises are true, therefore argument is valid.

Let B = Main course will be beef
    F = Main course will be fish
    P = Vegetable will be peas
    C = Vegetable will be corn

B ∨ F
P ∨ C
¬(F ∧ C)
--------
(B ∧ P)

| B | F | P | C | B ∨ F | P ∨ C | ¬(F ∧ C) | B ∧ P |    |
|---+---+---+---+-------+-------+----------+-------+----|
| F | F | F | F | F     | F     | T   F    | F     |    |
| F | F | F | T | F     | T     | T   F    | F     |    |
| F | F | T | F | F     | T     | T   F    | F     |    |
| F | F | T | T | F     | T     | T   F    | F     |    |
| F | T | F | F | T     | F     | T   F    | F     |    |
| F | T | F | T | T     | T     | F   T    | F     |    |
| F | T | T | F | T     | T     | T   F    | F     | :( |
| F | T | T | T | T     | T     | F   T    | F     |    |
| T | F | F | F | T     | F     | T   F    | F     |    |
| T | F | F | T | T     | T     | T   F    | F     | :( |
| T | F | T | F | T     | T     | T   F    | T     | :) |
| T | F | T | T | T     | T     | T   F    | T     | :) |
| T | T | F | F | T     | F     | T   F    | F     |    |
| T | T | F | T | T     | T     | F   T    | F     |    |
| T | T | T | F | T     | T     | T   F    | T     | :) |
| T | T | T | T | T     | T     | F   T    | T     |    |

There exists cases where all premises are true but conclusion is false therefore this is an invalid argument.

Let J = John is telling the truth
    B = Bill is telling the truth
    S = Sam is telling the truth

| J | B | S | J ∨ B | (¬S ∨ ¬B) | (J ∨ ¬S) |    |
|---+---+---+-------+-----------+----------+----|
| F | F | F | F     | T         | T        |    |
| F | F | T | F     | T         | F        |    |
| F | T | F | T     | T         | T        | :) |
| F | T | T | T     | F         | F        |    |
| T | F | F | T     | T         | T        |    |
| T | F | T | T     | T         | T        | :) |
| T | T | F | T     | T         | T        | :) |
| T | T | T | T     | F         | T        |    |

Conclusion is true when premises are true, therefore valid argument.

Let S = Sales go up
    X = Expenses go up
    B = Boss will be happy


| S | X | B | (S ∧ B) ∨ (X ∧ ¬B) | S \vert X |
|---+---+---+--------------------+-----------|
| F | F | F | F                  | T         |
| F | F | T | F                  | T         |
| F | T | F | T                  | F         |
| F | T | T | F                  | F         |
| T | F | F | F                  | F         |
| T | F | T | T                  | F         |
| T | T | F | T                  | F         |
| T | T | T | T                  | F         |

Argument is invalid because conclusion isn't always true when premise is true.

** Exercise 8

| P | Q | (P ∧ Q) ∨ (¬P ∧ ¬Q) | ¬P ∨ Q | (P ∨ ¬Q) ∧ (Q ∨ ¬P) | ¬(P ∨ Q) | (Q ∧ P) ∨ ¬P |
|---+---+---------------------+--------+---------------------+----------+--------------|
| F | F | T                   | T      | T                   | T        | T            |
| F | T | F                   | T      | F                   | F        | T            |
| T | F | F                   | F      | F                   | F        | F            |
| T | T | T                   | T      | T                   | F        | T            |

(Q ∧ P) ∨ ¬P and
(P ∨ ¬Q) ∧ (Q ∨ ¬P) are equivalent.

¬P ∨ Q and
(Q ∧ P) ∨ ¬P are equivalent.

** Exercise 9

a) Neither.
b) Contradiction.
c) Tautology.
d) Tautology.

** Exercise 10
